---
title: "CUNY 605"
subtitle: "Week 14 HW Assignment"
author: "mehtablocker"
date: "`r format(Sys.Date(), '%B %d, %Y')`"
output:
  html_document:
    toc: true
    toc_float: true
---

<style type="text/css">
h3 {
  color: DarkBlue;
}
</style>

```{r setup, include=FALSE}
knitr::opts_chunk$set(echo = TRUE)

```

<br>

__Taylor Series expansions__

<br>

###1

$$ f(x) = \frac{1}{(1-x)} $$
$$ f'(x) = \frac{1}{(1-x)^2} $$
$$ f''(x) = \frac{2}{(1-x)^3} $$
$$ f'''(x) = \frac{6}{(1-x)^4} $$
$$ f^{(n)}(x) = \frac{n!}{(1-x)^{n+1}} $$
$$ f^{(n)}(0) = n! $$
So, using Taylor Series formula...

$$ \frac{1}{(1-x)} = \sum \frac{f^{(n)}(0)}{n!}x^n $$
$$ = \sum \frac{n!}{n!}x^n $$
$$ = \sum_{n=0}^{\infty} x^n $$

###2

$$ f(x) = e^x $$
$$ f'(x) = e^x; f''(x) = e^x; f'''(x) = e^x $$
$$ f^{(n)}(x) = e^x $$
$$ f^{(n)}(0) = 1 $$
So, using Taylor Series formula...

$$ e^x = \sum \frac{f^{(n)}(0)}{n!}x^n $$
$$ = \sum \frac{1}{n!}x^n $$

###3

$$ f(x) = ln(1 + x) $$
$$ f'(x) = \frac{1}{(x + 1)} $$
$$ f''(x) = \frac{-1}{(x + 1)^2} $$
$$ f'''(x) = \frac{2}{(x + 1)^3} $$
$$ f''''(x) = \frac{-6}{(x + 1)^4} $$
$$ f^{(n)}(x) = \frac{(-1)^{n-1}(n-1)!}{(x + 1)^n} $$
$$ f^{(n)}(0) = (-1)^{n-1}(n-1)! $$
So, using Taylor Series formula...

$$ ln(x + 1) = \sum \frac{f^{(n)}(0)}{n!}x^n $$
$$ = \sum \frac{(-1)^{n-1}(n-1)!}{n!}x^n $$
And after a few steps...

$$ = x - \frac{x^2}{2} + \frac{x^3}{3} - \frac{x^4}{4} ... $$
